extraction/theories/ErasureCorrectness.v
@@ -16,7 +16,9 @@ From MetaCoq.Erasure Require Import EWcbvEval.
 From MetaCoq.Erasure Require Import Extract.
 From MetaCoq.PCUIC Require Import PCUICAstUtils.
 From MetaCoq.PCUIC Require Import PCUICInduction.
+From MetaCoq.PCUIC Require Import PCUICInversion.
 From MetaCoq.PCUIC Require Import PCUICSafeLemmata.
+From MetaCoq.PCUIC Require Import PCUICSR.
 From MetaCoq.PCUIC Require Import PCUICTyping.
 From MetaCoq.PCUIC Require Import PCUICWcbvEval.
 From MetaCoq.PCUIC Require Import PCUICWeakeningEnv.
@@ -126,7 +128,7 @@ Proof.
     constructor; [now apply f|now apply f'].
 Defined.
 
-Lemma erases_deps_cons Σ Σ' kn decl t :
+Lemma erases_deps_cons_left Σ Σ' kn decl t :
   wf ((kn, decl) :: Σ) ->
   erases_deps Σ Σ' t ->
   erases_deps ((kn, decl) :: Σ) Σ' t.
@@ -171,8 +173,370 @@ Proof.
   - easy.
 Qed.
 
+Lemma erases_deps_cons Σ Σ' kn decl decl' t :
+  wf ((kn, decl) :: Σ) ->
+  erases_deps Σ Σ' t ->
+  erases_deps ((kn, decl) :: Σ) ((kn, decl') :: Σ') t.
+Proof.
+  intros wfΣ er.
+  induction er using erases_deps_forall_ind; try solve [now constructor].
+  apply lookup_env_Some_fresh in H as not_fresh.
+  econstructor.
+  - unfold declared_constant in *.
+    cbn.
+    unfold eq_kername.
+    inversion wfΣ; subst.
+    destruct kername_eq_dec as [<-|]; [congruence|].
+    eassumption.
+  - unfold ETyping.declared_constant in *.
+    cbn.
+    inversion wfΣ; subst.
+    destruct kername_eq_dec; [congruence|].
+    eassumption.
+  - unfold erases_constant_body in *.
+    destruct PCUICAst.cst_body eqn:body.
+    + destruct E.cst_body eqn:ebody; [|easy].
+      assert (declared_constant ((kn, decl) :: Σ) kn0 cb).
+      { unfold declared_constant.
+        cbn.
+        unfold eq_kername.
+        inversion wfΣ; subst.
+        destruct kername_eq_dec as [<-|]; [congruence|].
+        easy. }
+      inversion wfΣ; subst.
+      eapply PCUICWeakeningEnv.declared_constant_inv in H4; eauto.
+      2:eapply PCUICWeakeningEnv.weaken_env_prop_typing.
+      red in H4.
+      rewrite body in *.
+      cbn in *.
+      eapply (erases_extends (_, P.cst_universes cb)); eauto.
+      2: eexists [_]; reflexivity.
+      eapply declared_constant_inv in H.
+      2:eapply PCUICWeakeningEnv.weaken_env_prop_typing.
+      2: easy.
+      2: easy.
+      unfold on_constant_decl in H.
+      rewrite body in *.
+      apply H.
+    + now destruct E.cst_body.
+  - easy.
+Qed.
+
+Lemma In_add_seen k k' ks :
+  (k = k' \/ In k ks) ->
+  In k (add_seen k' ks).
+Proof.
+  intros [->|].
+  - unfold add_seen.
+    destruct existsb eqn:ex; [|now left].
+    apply existsb_exists in ex as (k & ? & ?).
+    unfold eq_kername in *.
+    now destruct kername_eq_dec as [<-|].
+  - unfold add_seen.
+    destruct existsb eqn:ex; [easy|].
+    now right.
+Qed.
+
+Lemma In_box_type_deps k ks t :
+  In k ks ->
+  In k (box_type_deps ks t).
+Proof.
+  intros isin.
+  induction t in ks, t, isin |- *; cbn in *; auto.
+  - now apply In_add_seen.
+  - now apply In_add_seen.
+Qed.
+
+Lemma In_fold_left {A} k (ks : list kername) f (ts : list A) :
+  In k ks ->
+  (forall a ks, In a ts -> In k ks -> In k (f ks a)) ->
+  In k (fold_left f ts ks).
+Proof.
+  intros isin allin.
+  induction ts in ks, ts, isin, allin |- *; [easy|].
+  apply IHts.
+  - apply allin; [|easy].
+    now left.
+  - intros.
+    apply allin; [|easy].
+    now right.
+Qed.
+
+Lemma In_Eterm_deps k ks t :
+  In k ks ->
+  In k (Eterm_deps ks t).
+Proof.
+  intros isin.
+  induction t in ks, t, isin |- * using EInduction.term_forall_list_ind; cbn in *; auto.
+  - induction H in ks, isin |- *; [easy|].
+    cbn in *.
+    now apply IHForall.
+  - now apply In_add_seen.
+  - now apply In_add_seen.
+  - destruct p.
+    apply In_fold_left.
+    + now apply IHt, In_add_seen.
+    + intros.
+      destruct a.
+      now eapply All_In in H as [H]; [|eassumption].
+  - destruct s as ((ind & npars) & arg).
+    now apply IHt, In_add_seen.
+  - apply In_fold_left; [easy|].
+    intros.
+    now eapply Forall_All, All_In in H as [H]; [|eassumption].
+  - apply In_fold_left; [easy|].
+    intros.
+    now eapply Forall_All, All_In in H as [H]; [|eassumption].
+Qed.
+
+Lemma In_fold_box_type_deps k ks ts :
+  In k ks ->
+  In k (fold_left box_type_deps ts ks).
+Proof.
+  intros isin.
+  induction ts in ks, ts, isin |- *; [easy|].
+  now apply IHts, In_box_type_deps.
+Qed.
+
+Lemma In_decl_deps k ks decl :
+  In k ks ->
+  In k (decl_deps ks decl).
+Proof.
+  intros isin.
+  destruct decl; cbn in *.
+  - apply In_box_type_deps.
+    destruct ExAst.cst_body; [|easy].
+    now apply In_Eterm_deps.
+  - apply In_fold_left; [easy|].
+    intros.
+    apply In_fold_left.
+    + apply In_fold_left; [easy|].
+      intros.
+      now eapply In_box_type_deps.
+    + intros.
+      now apply In_box_type_deps.
+  - destruct p.
+    now apply In_box_type_deps.
+Qed.
+
+Lemma erases_forall_list_ind :
+forall (Σ : PCUICAst.global_env_ext)
+  (P : PCUICAst.context -> PCUICAst.term -> Extract.E.term -> Prop),
+(forall (Γ : PCUICAst.context) (i : nat), P Γ (PCUICAst.tRel i) (Extract.E.tRel i)) ->
+(forall (Γ : PCUICAst.context) (n : ident), P Γ (PCUICAst.tVar n) (Extract.E.tVar n)) ->
+(forall (Γ : PCUICAst.context) (m m' : nat) (l : list PCUICAst.term) (l' : list Extract.E.term),
+ All2 (erases Σ Γ) l l' ->
+ Forall2 (P Γ) l l' ->
+ P Γ (PCUICAst.tEvar m l) (Extract.E.tEvar m' l')) ->
+(forall (Γ : PCUICAst.context) (na : name) (b t : PCUICAst.term) (t' : Extract.E.term),
+ Σ;;; (PCUICAst.vass na b :: Γ) |- t ⇝ℇ t' ->
+ P (PCUICAst.vass na b :: Γ) t t' -> P Γ (PCUICAst.tLambda na b t) (Extract.E.tLambda na t')) ->
+(forall (Γ : PCUICAst.context) (na : name) (t1 : PCUICAst.term) (t1' : Extract.E.term)
+   (T t2 : PCUICAst.term) (t2' : Extract.E.term),
+ Σ;;; Γ |- t1 ⇝ℇ t1' ->
+ P Γ t1 t1' ->
+ Σ;;; (PCUICAst.vdef na t1 T :: Γ) |- t2 ⇝ℇ t2' ->
+ P (PCUICAst.vdef na t1 T :: Γ) t2 t2' ->
+ P Γ (PCUICAst.tLetIn na t1 T t2) (Extract.E.tLetIn na t1' t2')) ->
+(forall (Γ : PCUICAst.context) (f4 u : PCUICAst.term) (f' u' : Extract.E.term),
+ Σ;;; Γ |- f4 ⇝ℇ f' ->
+ P Γ f4 f' -> Σ;;; Γ |- u ⇝ℇ u' -> P Γ u u' -> P Γ (PCUICAst.tApp f4 u) (Extract.E.tApp f' u')) ->
+(forall (Γ : PCUICAst.context) (kn : kername) (u : Universes.Instance.t),
+ P Γ (PCUICAst.tConst kn u) (Extract.E.tConst kn)) ->
+(forall (Γ : PCUICAst.context) (kn : inductive) (k : nat) (n : Universes.Instance.t),
+ P Γ (PCUICAst.tConstruct kn k n) (Extract.E.tConstruct kn k)) ->
+(forall (Γ : PCUICAst.context) (ind : inductive) (npar : nat) (T c : PCUICAst.term)
+   (brs : list (nat × PCUICAst.term)) (c' : Extract.E.term) (brs' : list (nat × Extract.E.term)),
+ PCUICElimination.Informative Σ ind ->
+ Σ;;; Γ |- c ⇝ℇ c' ->
+ P Γ c c' ->
+ All2
+   (fun (x : nat × PCUICAst.term) (x' : nat × Extract.E.term) => Σ;;; Γ |- x.2 ⇝ℇ x'.2 × x.1 = x'.1)
+   brs brs' ->
+Forall2 (fun br br' => P Γ br.2 br'.2) brs brs' ->
+ P Γ (PCUICAst.tCase (ind, npar) T c brs) (Extract.E.tCase (ind, npar) c' brs')) ->
+(forall (Γ : PCUICAst.context) (p : (inductive × nat) × nat) (c : PCUICAst.term)
+   (c' : Extract.E.term),
+ let ind := p.1.1 in
+ PCUICElimination.Informative Σ ind ->
+ Σ;;; Γ |- c ⇝ℇ c' -> P Γ c c' -> P Γ (PCUICAst.tProj p c) (Extract.E.tProj p c')) ->
+(forall (Γ : PCUICAst.context) (mfix : mfixpoint PCUICAst.term) (n : nat)
+   (mfix' : list (Extract.E.def Extract.E.term)),
+ All2
+   (fun (d : def PCUICAst.term) (d' : Extract.E.def Extract.E.term) =>
+    dname d = Extract.E.dname d'
+    × rarg d = Extract.E.rarg d'
+      × Σ;;; PCUICAst.app_context Γ (PCUICLiftSubst.fix_context mfix) |-
+        dbody d ⇝ℇ Extract.E.dbody d') mfix mfix' ->
+ Forall2 (fun d d' => P (PCUICAst.app_context Γ (PCUICLiftSubst.fix_context mfix)) (dbody d) (EAst.dbody d') ) mfix mfix' ->
+ P Γ (PCUICAst.tFix mfix n) (Extract.E.tFix mfix' n)) ->
+(forall (Γ : PCUICAst.context) (mfix : mfixpoint PCUICAst.term) (n : nat)
+   (mfix' : list (Extract.E.def Extract.E.term)),
+ All2
+   (fun (d : def PCUICAst.term) (d' : Extract.E.def Extract.E.term) =>
+    dname d = Extract.E.dname d'
+    × rarg d = Extract.E.rarg d'
+      × Σ;;; PCUICAst.app_context Γ (PCUICLiftSubst.fix_context mfix) |-
+        dbody d ⇝ℇ Extract.E.dbody d') mfix mfix' ->
+ Forall2 (fun d d' => P (PCUICAst.app_context Γ (PCUICLiftSubst.fix_context mfix)) (dbody d) (EAst.dbody d') ) mfix mfix' ->
+ P Γ (PCUICAst.tCoFix mfix n) (Extract.E.tCoFix mfix' n)) ->
+(forall (Γ : PCUICAst.context) (t : PCUICAst.term), isErasable Σ Γ t -> P Γ t Extract.E.tBox) ->
+forall (Γ : PCUICAst.context) (t : PCUICAst.term) (t0 : Extract.E.term),
+Σ;;; Γ |- t ⇝ℇ t0 -> P Γ t t0.
+Proof.
+  intros until t0.
+
+Lemma erases_deps_recursive Σ Σer t T et :
+  wf_ext Σ ->
+  Σ;;; [] |- t : T ->
+  Σ;;; [] |- t ⇝ℇ et ->
+  (forall k,
+      In k (Eterm_deps [] et) ->
+      match P.lookup_env Σ k with
+      | Some (P.ConstantDecl _) => erases_deps Σ Σer (E.tConst k)
+      | _ => True
+      end) ->
+  erases_deps Σ Σer et.
+Proof.
+  intros wf wt er deps_er.
+  induction er in t, T, et, wf, wt, er, deps_er |- * using erases_forall_list_ind; cbn in *.
+  - now constructor.
+  - now constructor.
+  - now apply inversion_Evar in wt.
+  - constructor.
+    apply inversion_Lambda in wt as (? & ? & ? & ? & ?); eauto.
+  - apply inversion_LetIn in wt as (? & ? & ? & ? & ? & ?); eauto.
+    constructor.
+    + eapply IHer1; eauto.
+      intros.
+      apply deps_er.
+      now apply In_Eterm_deps.
+    + eapply IHer2; eauto.
+      intros.
+      apply deps_er.
+      admit.
+  - apply inversion_App in wt as (? & ? & ? & ? & ? & ?); eauto.
+    constructor.
+    + eapply IHer1; eauto.
+      intros.
+      apply deps_er.
+      now apply In_Eterm_deps.
+    + eapply IHer2; eauto.
+      intros.
+      apply deps_er.
+      admit.
+  - apply inversion_Const in wt as (? & ? & ? & ? & ?); eauto.
+    specialize (deps_er kn (or_introl eq_refl)).
+    unfold declared_constant in d.
+    unfold PCUICAst.fst_ctx, fst_ctx in *.
+    now rewrite d in deps_er.
+  - now constructor.
+  - apply inversion_Case in wt
+      as (? & ? & ? & ? & ? & ? & ? & ? & ? & ? & ? & ? & ? & ? & ? & ? & ?); eauto.
+    constructor.
+    + eapply IHer; eauto.
+      intros.
+      eapply deps_er.
+      apply In_fold_left.
+      * admit.
+      * intros.
+        destruct a0.
+        now apply In_Eterm_deps.
+    + clear -wf a X H0 deps_er.
+      revert a X H0 deps_er.
+      generalize brs' at 3.
+      intros brs_gen.
+      revert brs' x5.
+      induction brs; intros brs' brtys typ er all_deps deps.
+      { now depelim er. }
+      depelim typ.
+      depelim er.
+      depelim all_deps.
+      destruct p as ((? & ?) & ?).
+      destruct p0.
+      constructor.
+      * eapply H; eauto.
+        intros.
+        apply deps.
+        cbn.
+        destruct y0; cbn in *.
+        apply In_fold_left.
+        -- admit.
+        -- intros.
+           destruct a0.
+           now apply In_Eterm_deps.
+      * eapply IHbrs; eauto.
+
+  - apply inversion_Proj in wt as (?&?&?&?&?&?&?&?&?); eauto.
+    constructor.
+    eapply IHer; eauto.
+    intros; apply deps_er.
+    destruct p as ((? & ?) & ?).
+    admit.
+  - constructor.
+    apply inversion_Fix in wt as (?&?&?&?&?&?&?); eauto.
+    clear -wf a0 X H deps_er.
+    revert a0 X H deps_er.
+    generalize mfix at 1 2 4 6.
+    intros mfix_gen.
+    revert mfix'.
+    induction mfix; cbn in *; intros mfix' typ er all_deps deps.
+    { now depelim er. }
+    depelim typ.
+    depelim er.
+    depelim all_deps.
+    destruct p.
+    destruct p0 as (?&?&?).
+    constructor.
+    + eapply H; eauto.
+      intros.
+      apply deps.
+      cbn in *.
+      apply In_fold_left; [easy|].
+      intros.
+      now apply In_Eterm_deps.
+    + apply IHmfix; eauto.
+      intros.
+      apply deps.
+      cbn in *.
+      admit.
+  - constructor.
+    apply inversion_CoFix in wt as (?&?&?&?&?&?&?); eauto.
+    clear -wf a0 X H deps_er.
+    revert a0 X H deps_er.
+    generalize mfix at 1 2 4 6.
+    intros mfix_gen.
+    revert mfix'.
+    induction mfix; cbn in *; intros mfix' typ er all_deps deps.
+    { now depelim er. }
+    depelim typ.
+    depelim er.
+    depelim all_deps.
+    destruct p as (?&?&?).
+    constructor.
+    + eapply H; eauto.
+      intros.
+      apply deps.
+      cbn in *.
+      apply In_fold_left; [easy|].
+      intros.
+      now apply In_Eterm_deps.
+    + apply IHmfix; eauto.
+      intros.
+      apply deps.
+      cbn in *.
+      admit.
+  - now constructor.
+Admitted.
+
+Opaque erase_type SafeErasureFunction.wf_reduction.
 Lemma erase_global_decls_deps_recursive_correct Σ wfΣ include ignore erase_func Σex :
   (forall k, ignore k = false) ->
+  (forall Σ Γ t T wfΣ t',
+      Σ;;; Γ |- t : T ->
+      forall wt,
+        erase_func Σ wfΣ Γ t wt = PCUICSafeChecker.Checked t' ->
+        Σ;;; Γ |- t ⇝ℇ t') ->
   erase_global_decls_deps_recursive erase_func Σ wfΣ include ignore = Ok Σex ->
   (forall k,
       In k include ->
@@ -182,25 +546,19 @@ Lemma erase_global_decls_deps_recursive_correct Σ wfΣ include ignore erase_fun
       | _ => True
       end).
 Proof.
-Ltac unproof :=
-  repeat
-    multimatch goal with
-    | [H: context[erase_global_decl _ _ ?wfΣ _ _ _ ?wfdecl] |- _] =>
-      first
-        [is_var wfΣ|
-         (let wfΣid := fresh "wfΣ" in set (wfΣid := wfΣ) in *; clearbody wfΣid)];
-      first
-        [is_var wfdecl|
-         (let wfdeclid := fresh "wfdecl" in set (wfdeclid := wfdecl) in *; clearbody wfdeclid)]
-    | [H: context[erase_global_decls_deps_recursive _ _ ?wfΣ] |- _] =>
-      first
-        [is_var wfΣ|
-         (let wfΣid := fresh "wfΣ" in set (wfΣid := wfΣ) in *; clearbody wfΣid)]
-    end.
-
-  intros no_ignores er.
+  intros no_ignores erase_erases er.
   induction Σ as [|(kn, decl) Σ IH] in wfΣ, include, Σex, er |- *; [easy|].
-  cbn in *; unproof.
+  cbn in *.
+  match goal with
+  | [H: context[erase_global_decl _ _ ?wfΣarg _ _ _ ?wfdeclarg] |- _] =>
+      set (wfΣext := wfΣarg) in *; clearbody wfΣext;
+        set (wfdecl := wfdeclarg) in *; clearbody wfdecl
+  end.
+  match goal with
+  | [H: context[erase_global_decls_deps_recursive _ _ ?wfΣarg] |- _] =>
+    set (wfΣprev := wfΣarg) in *; clearbody wfΣprev
+  end.
+
   rewrite no_ignores in er.
   destruct (contains kn include) eqn:contains; cycle 1.
   - cbn in *.
@@ -212,55 +570,106 @@ Ltac unproof :=
     + destruct P.lookup_env; [|easy].
       destruct g; [|easy].
       destruct wfΣ.
-      now apply erases_deps_cons.
+      now apply erases_deps_cons_left.
   - cbn in *.
     destruct erase_global_decl eqn:erdecl; cbn in *; [|congruence].
     destruct erase_global_decls_deps_recursive eqn:errec; [|congruence].
     inversion er; subst; clear er.
     intros k isin.
     unfold eq_kername.
-    destruct kername_eq_dec as [->|].
-    + destruct decl; [|easy].
-      econstructor.
-      * unfold declared_constant; cbn.
-        rewrite eq_kername_refl.
-        reflexivity.
-      * simpl in erdecl.
-
-    eapply IH in errec.
-  - cbn in *.
-    destruct erase_global_decl eqn:erdecl; [|congruence].
-    inversion er; subst; clear er.
-    cbn in *.
-    destruct decl; cycle 1.
-    * simpl in erdecl.
-  rew
-  destruct P.lookup_env eqn:lookup; [|easy].
-  destruct g; [|easy].
-  cbn in *; unproof.
-  Admitted.
-(*  cbn.
-  cbn in *; unproof.
-  rewrite no_ignores in er.
-  destruct (contains kn include) eqn:contains.
-  - cbn in *.
-    destruct erase_global_decl eqn:erdecl; [|congruence].
-    destruct erase_global_decls_deps_recursive eqn:errec; [|congruence].
-    inversion er; subst; clear er.
-    cbn in *.
-    destruct decl; cycle 1.
-    * simpl in erdecl.
-      destruct erase_ind; simpl in *; [|congruence].
+    destruct kername_eq_dec as [->|]; cycle 1.
+    { cbn in *.
+      eapply IH with (k := k) in errec; eauto.
+      destruct P.lookup_env; [|easy].
+      destruct g; [|easy].
+      destruct wfΣ.
+      destruct t;
+        eauto using erases_deps_cons, erases_deps_cons_left.
+      now apply In_decl_deps. }
+    destruct decl; [|easy].
+    cbn -[erase_constant_decl] in *.
+    destruct erase_constant_decl eqn:erconst; cbn -[erase_constant_decl] in *; [|congruence].
+    unfold erase_constant_decl in erconst.
+    destruct flag_of_type; cbn in *; [|congruence].
+    destruct a; cbn in *.
+    destruct is_sort.
+    + cbn in wfdecl.
+      destruct c.
+      destruct cst_body; cbn in *; [|congruence].
+      destruct erase_type; cbn in *; [|congruence].
+      inversion erconst; subst; clear erconst.
       inversion erdecl; subst; clear erdecl.
-      simpl in *.
-      eapply IH in errec.
-    * cbn.
-      constructor.
+      cbn in *.
+      econstructor.
+      * unfold declared_constant; cbn; rewrite eq_kername_refl.
+        reflexivity.
+      * unfold ETyping.declared_constant; cbn.
+        destruct kername_eq_dec; [|congruence].
+        reflexivity.
+      * cbn.
+        destruct wfΣ as [wfΣ].
+        destruct wfdecl as [wfdecl].
+        destruct i as (u & [redu]).
+        eapply type_reduction in wfdecl; eauto.
+        2: now inversion wfΣ.
+        constructor.
+        eapply (Is_type_extends (Σ, _)).
+        2: now eauto.
+        2: eexists [_]; reflexivity.
+        1: now eauto.
+        eexists _.
+        split; [eassumption|].
+        now left.
+      * intros.
+        cbn in *.
+        inversion H; subst; clear H.
+        now constructor.
+    + destruct erase_type; cbn in *; [|congruence].
+      destruct c; cbn in *.
+      destruct cst_body; cycle 1.
+      { inversion erconst; subst; clear erconst.
+        inversion erdecl; subst; clear erdecl.
+        cbn in *.
+        econstructor.
+        - unfold declared_constant; cbn; rewrite eq_kername_refl; reflexivity.
+        - unfold ETyping.declared_constant; cbn.
+          destruct kername_eq_dec; [|congruence].
+          reflexivity.
+        - easy.
+        - intros.
+          cbn in *.
+          congruence. }
 
-  econstructor.
-  - easy.
-  -
-  eapply erases_deps_tConst.
-  er : erase_global_decls_deps_recursive SafeErasureFunction.erase Σ (wf_ext_wf_squash wfΣ) [kn]
-         (fun _ : kername => false) = Ok Σex
-*)
+      destruct erase_func eqn:er; cbn in *; [|congruence].
+      inversion erconst; subst; clear erconst.
+      inversion erdecl; subst; clear erdecl.
+      cbn in *.
+      specialize (IH _ _ _ errec).
+      destruct wfΣ as [wfΣ].
+      destruct wfdecl as [wfdecl].
+      eapply erase_erases in er; eauto.
+      econstructor.
+      * unfold declared_constant; cbn; rewrite eq_kername_refl; reflexivity.
+      * unfold ETyping.declared_constant; cbn.
+        destruct kername_eq_dec; [|congruence].
+        reflexivity.
+      * cbn.
+        eapply type_reduction in wfdecl; eauto.
+        2: now inversion wfΣ.
+        eapply (erases_extends (_, _)).
+        2: eauto.
+        1: now inversion wfΣ.
+        2: eexists [_]; reflexivity.
+        2: eauto.
+        eauto.
+      * intros.
+        cbn in *.
+        noconf H.
+        destruct wfΣext.
+        apply erases_deps_cons; eauto.
+        eapply (erases_deps_recursive (Σ, cst_universes)); eauto.
+        intros.
+        apply IH.
+        apply In_box_type_deps.
+        todo "easy".
+Qed.
